src/HOL/ex/Classpackage.thy
@@ -26,7 +26,7 @@ proof
   from semigroup_int_def show "k \<otimes> l \<otimes> j = k \<otimes> (l \<otimes> j)" by simp
 qed
 
-instance (type) list :: semigroup
+instance list :: (type) semigroup
   "xs \<otimes> ys \<equiv> xs @ ys"
 proof
   fix xs ys zs :: "'a list"
@@ -52,7 +52,7 @@ next
   from monoidl_num_def show "\<one> \<otimes> k = k" by simp
 qed
 
-instance (type) list :: monoidl
+instance list :: (type) monoidl
   "\<one> \<equiv> []"
 proof
   fix xs :: "'a list"
@@ -67,7 +67,7 @@ qed
 class monoid = monoidl +
   assumes neutr: "x \<^loc>\<otimes> \<^loc>\<one> = x"
 
-instance monoid_list_def: (type) list :: monoid
+instance monoid_list_def: list :: (type) monoid
 proof
   fix xs :: "'a list"
   show "xs \<otimes> \<one> = xs"
@@ -288,26 +288,26 @@ lemma (in group) int_pow_one:
   "\<^loc>\<one> \<^loc>\<up> (k\<Colon>int) = \<^loc>\<one>"
 using pow_def nat_pow_one inv_one by simp
 
-instance semigroup_prod_def: (semigroup, semigroup) * :: semigroup
+instance semigroup_prod_def: * :: (semigroup, semigroup) semigroup
   mult_prod_def: "x \<otimes> y \<equiv> let (x1, x2) = x; (y1, y2) = y in
               (x1 \<otimes> y1, x2 \<otimes> y2)"
 by default (simp_all add: split_paired_all semigroup_prod_def assoc)
 
-instance monoidl_prod_def: (monoidl, monoidl) * :: monoidl
+instance monoidl_prod_def: * :: (monoidl, monoidl) monoidl
   one_prod_def: "\<one> \<equiv> (\<one>, \<one>)"
 by default (simp_all add: split_paired_all monoidl_prod_def neutl)
 
-instance monoid_prod_def: (monoid, monoid) * :: monoid
+instance monoid_prod_def: * :: (monoid, monoid) monoid
 by default (simp_all add: split_paired_all monoid_prod_def neutr)
 
-instance monoid_comm_prod_def: (monoid_comm, monoid_comm) * :: monoid_comm
+instance monoid_comm_prod_def: * :: (monoid_comm, monoid_comm) monoid_comm
 by default (simp_all add: split_paired_all monoidl_prod_def comm)
 
-instance group_prod_def: (group, group) * :: group
+instance group_prod_def: * :: (group, group) group
   inv_prod_def: "\<div> x \<equiv> let (x1, x2) = x in (\<div> x1, \<div> x2)"
 by default (simp_all add: split_paired_all group_prod_def invl)
 
-instance group_comm_prod_def: (group_comm, group_comm) * :: group_comm
+instance group_comm_prod_def: * :: (group_comm, group_comm) group_comm
 by default (simp_all add: split_paired_all group_prod_def comm)
 
 definition
